ts: rename Path.lean to PathFragment.lean

CTL/Basic.lean
@@ -1,6 +1,12 @@
-variable {p : Type}
+import TS.Basic
+import TS.PathFragment
+import CTL.Satisfaction
+import CTL.Equivalence
 
 namespace CTL
+open TS
+variable {p : Type}
+
 mutual
   inductive StateFormula where
     | top   : StateFormula
@@ -39,7 +45,6 @@ namespace StateFormula
   def potentialAll := neg (inevitable (neg Φ))
   @[simp]
   def invariant    := neg (potential (neg Φ))
-end StateFormula
 
 namespace Syntax
   notation  "⬝⊤"   => StateFormula.top
@@ -59,4 +64,128 @@ namespace Syntax
   prefix:50 "⬝◯"   => PathFormula.next
   infixr:50 " ⬝U " => PathFormula.untl
 end Syntax
+
+section Satisfaction
+variable {inst : Fintype s}
+mutual
+  -- s ⊨ Φ
+  @[simp]
+  def StateSat (ts : TS s a p) (st : s) :=
+    fun
+      | StateFormula.top => True
+      | ⬝a               => a ∈ ts.label st
+      | ⬝¬Φ              => ¬(StateSat ts st Φ)
+      | Φ₁ ⬝∧ Φ₂         => (StateSat ts st Φ₁) ∧ (StateSat ts st Φ₂)
+      | ⬝∃ φ             => ∃ π : TS.PathFragment.From ts st, PathSat ts π.1.2 φ
+      | ⬝∀ φ             => ∀ π : TS.PathFragment.From ts st, PathSat ts π.1.2 φ
+
+  -- π ⊨ φ
+  @[simp]
+  def PathSat (ts : TS s a p) (π : ts.PathFragment n) :=
+    fun
+      | ⬝◯ Φ   => StateSat ts (π.second) Φ
+      | Φ ⬝U Ψ => ∃ j : EFin (Order.succ n), (StateSat ts (π.get j) Ψ) ∧ ∀ k : EFin j.val, StateSat ts (π.get (EFin.castLT j.lt k)) Φ
+end
+
+instance : StateSatisfiable p (@StateFormula p) where
+  StateSat := StateSat
+
+@[simp]
+theorem StateSat_potentialAll {st : s} : StateSat ts st (⬝∃■Φ) ↔ ∃π : TS.PathFragment.From ts st, ∀j, StateSat ts (π.1.2.get j) Φ := by
+  simp
+
+@[simp]
+theorem StateStat_invariant : StateSat ts st (⬝∀■Φ) ↔ ∀π : TS.PathFragment.From ts st, ∀j, StateSat ts (π.1.2.get j) Φ := by
+  simp
+end Satisfaction
+
+section Equiv
+variable {Φ Φ' Φ₁ Φ₁' Φ₂ Φ₂' Ψ Ψ' : @StateFormula p}
+
+@[simp]
+theorem conj_congr (h₁ : Equiv (p := p) Φ₁ Φ₁') (h₂ : Equiv (p := p) Φ₂ Φ₂') : Equiv (p := p) (Φ₁ ⬝∧ Φ₂) (Φ₁' ⬝∧ Φ₂') := by
+  simp [Equiv, setOfSatStates, SatState, StateSatisfiable.StateSat, Set.ext_iff] at *
+  intros _ _ _ _ _
+  constructor
+  . rintro ⟨sat₁, sat₂⟩; constructor; exact (h₁ _).1 sat₁; exact (h₂ _).1 sat₂
+  . rintro ⟨sat₁, sat₂⟩; constructor; exact (h₁ _).2 sat₁; exact (h₂ _).2 sat₂
+
+@[simp]
+theorem neg_congr (h : Equiv (p := p) Φ Φ') : Equiv (p := p) (⬝¬Φ) (⬝¬Φ') := by
+  simp [Equiv, setOfSatStates, SatState, StateSatisfiable.StateSat, Set.ext_iff] at *
+  intros _ _ _ _ _
+  constructor
+  . rintro negSat sat; exact negSat ((h _).2 sat)
+  . rintro negSat sat; exact negSat ((h _).1 sat)
+
+@[simp]
+theorem exist_next_congr (h : Equiv (p := p) Φ Φ') : Equiv (p := p) (⬝∃⬝◯Φ) (⬝∃⬝◯Φ') := by
+  simp [Equiv, setOfSatStates, SatState, StateSatisfiable.StateSat, Set.ext_iff] at *
+  intros _ _ _ _ _
+  constructor
+  . rintro ⟨π, sat⟩; exact ⟨π, (h _).1 sat⟩
+  . rintro ⟨π, sat⟩; exact ⟨π, (h _).2 sat⟩
+
+@[simp]
+theorem exist_untl_congr (h₁ : Equiv (p := p) Φ Φ') (h₂ : Equiv (p := p) Ψ Ψ') : Equiv (p := p) (⬝∃(Φ ⬝U Ψ)) (⬝∃(Φ' ⬝U Ψ')) := by
+  simp [Equiv, setOfSatStates, SatState, StateSatisfiable.StateSat, Set.ext_iff] at *
+  intros _ _ _ _ _
+  constructor
+  . rintro ⟨π, j, ⟨satJ, satK⟩⟩; exact ⟨π, j, ⟨(h₂ _).1 satJ, fun k => (h₁ _).1 (satK k)⟩⟩
+  . rintro ⟨π, j, ⟨satJ, satK⟩⟩; exact ⟨π, j, ⟨(h₂ _).2 satJ, fun k => (h₁ _).2 (satK k)⟩⟩
+
+@[simp]
+theorem all_next_congr (h : Equiv (p := p) Φ Φ') : Equiv (p := p) (⬝∀⬝◯Φ) (⬝∀⬝◯Φ') := by
+  simp [Equiv, setOfSatStates, SatState, StateSatisfiable.StateSat, Set.ext_iff] at *
+  intros _ _ _ _ _
+  constructor
+  . rintro sat π; rw [← h]; exact sat π
+  . rintro sat π; rw [h]  ; exact sat π
+  done
+
+@[simp]
+theorem all_untl_congr (h₁ : Equiv (p := p) Φ Φ') (h₂ : Equiv (p := p) Ψ Ψ') : Equiv (p := p) (⬝∀(Φ ⬝U Ψ)) (⬝∀(Φ' ⬝U Ψ')) := by
+  simp [Equiv, setOfSatStates, SatState, StateSatisfiable.StateSat, Set.ext_iff] at *
+  intros _ _ _ _ _
+  constructor
+  . rintro sat π; obtain ⟨j, ⟨satJ, satK⟩⟩ := sat π; exact ⟨j, ⟨(h₂ _).1 satJ, fun k => (h₁ _).1 (satK k)⟩⟩
+  . rintro sat π; obtain ⟨j, ⟨satJ, satK⟩⟩ := sat π; exact ⟨j, ⟨(h₂ _).2 satJ, fun k => (h₁ _).2 (satK k)⟩⟩
+
+theorem all_next_duality : Equiv (p := p) (⬝∀⬝◯Φ) (⬝¬(⬝∃⬝◯⬝¬Φ)) := by
+  simp [Equiv, setOfSatStates, SatState, StateSatisfiable.StateSat, Set.ext_iff] at *
+
+theorem inevitable_duality : Equiv (p := p) (⬝∀♢Φ) (⬝¬(⬝∃■⬝¬Φ)) := by
+  simp [Equiv, setOfSatStates, SatState, StateSatisfiable.StateSat, StateFormula.inevitable, PathFormula.untl]
+
+theorem exist_next_duality : Equiv (p := p) (⬝∃⬝◯Φ) (⬝¬(⬝∀⬝◯⬝¬Φ)) := by
+  simp [Equiv, setOfSatStates, SatState, StateSatisfiable.StateSat]
+
+theorem potential_duality : Equiv (p := p) (⬝∃♢Φ) (⬝¬(⬝∀■⬝¬Φ)) := by
+  simp [Equiv, setOfSatStates, SatState, StateSatisfiable.StateSat, StateFormula.potential, PathFormula.untl]
+
+theorem all_untl_duality : Equiv (p := p) (⬝∀(Φ ⬝U Ψ)) (⬝¬(⬝∃(⬝¬Ψ ⬝U (⬝¬Φ ⬝∧ ⬝¬Ψ))) ⬝∧ ⬝¬(⬝∃■⬝¬Ψ)) := by
+  simp [Equiv, setOfSatStates, SatState, StateSatisfiable.StateSat, Set.ext_iff] at *
+  intros _ _ _ _ _
+  constructor
+  . rintro sat
+    constructor
+    . rintro π j negSatΦ negSatΨ
+      obtain ⟨a, ⟨satΨ, satΦ⟩⟩ := sat π
+      sorry
+    . rintro π
+      obtain ⟨_, ⟨_, _⟩⟩ := sat π
+      constructor <;> assumption
+  . rintro ⟨negSat, satΨ⟩ π
+    obtain ⟨j, satΨ'⟩ := satΨ π
+    exact ⟨j, ⟨satΨ', fun k => sorry⟩⟩
+
+theorem all_untl_expansion : Equiv (p := p) (⬝∀(Φ ⬝U Ψ)) (Ψ ⬝∨ (Φ ⬝∧ (⬝∀⬝◯⬝∀(Φ ⬝U Ψ)))) := by
+  -- simp [Equiv, satStateSet, SatState, StateSat, PathSat, StateFormula.disj]
+  -- intro s a ts
+  -- ext x
+  -- done
+  sorry
+
+end Equiv
+end StateFormula
 end CTL
