CTL/Satisfaction.lean
@@ -1,7 +1,4 @@
-import CTL.Basic
 import TS.Basic
-import TS.Path
-import TS.EFin
 
 namespace CTL
 open TS
@@ -44,43 +41,4 @@ theorem Sat_iff_initial_subset {s a : Type} {_ : Fintype s} (ts : TS s a p) (Φ 
       obtain ⟨stSat, refl⟩ := sub
       rw [← refl]
       exact Subtype.property stSat
-
-
-namespace StateFormula
-variable (Φ Φ₁ Φ₂ : @StateFormula p)
-         (φ φ₁ φ₂ : @PathFormula p)
-         {inst : Fintype s}
-
-mutual
-  -- s ⊨ Φ
-  @[simp]
-  def StateSat (ts : TS s a p) (st : s) :=
-    fun
-      | StateFormula.top => True
-      | ⬝a               => a ∈ ts.label st
-      | ⬝¬Φ              => ¬(StateSat ts st Φ)
-      | Φ₁ ⬝∧ Φ₂         => (StateSat ts st Φ₁) ∧ (StateSat ts st Φ₂)
-      | ⬝∃ φ             => ∃ π : PathFragment.From ts st, PathSat ts π.1.2 φ
-      | ⬝∀ φ             => ∀ π : PathFragment.From ts st, PathSat ts π.1.2 φ
-
-  -- π ⊨ φ
-  @[simp]
-  def PathSat (ts : TS s a p) (π : ts.PathFragment n) :=
-    fun
-      | ⬝◯ Φ   => StateSat ts (π.second) Φ
-      | Φ ⬝U Ψ => ∃ j : EFin (Order.succ n), (StateSat ts (π.get j) Ψ) ∧ ∀ k : EFin j.val, StateSat ts (π.get (EFin.castLT j.lt k)) Φ
-end
-
-instance : StateSatisfiable p (@StateFormula p) where
-  StateSat := StateSat
-
-@[simp]
-theorem StateSat_potentialAll {st : s} : StateSat ts st (⬝∃■Φ) ↔ ∃π : PathFragment.From ts st, ∀j, StateSat ts (π.1.2.get j) Φ := by
-  simp
-
-@[simp]
-theorem StateStat_invariant : StateSat ts st (⬝∀■Φ) ↔ ∀π : PathFragment.From ts st, ∀j, StateSat ts (π.1.2.get j) Φ := by
-  simp
-
-end StateFormula
 end CTL
