CTL/Equivalence.lean
@@ -1,5 +1,4 @@
 import TS.Basic
-import CTL.Basic
 import CTL.Satisfaction
 
 namespace CTL
@@ -40,93 +39,5 @@ instance : IsPreorder α (Equiv (p := p)) where
 
 instance : IsEquiv α (Equiv (p := p)) where
 
-namespace StateFormula
-variable {Φ Φ' Φ₁ Φ₁' Φ₂ Φ₂' Ψ Ψ' : @StateFormula p}
-
-@[simp]
-theorem conj_congr (h₁ : Equiv (p := p) Φ₁ Φ₁') (h₂ : Equiv (p := p) Φ₂ Φ₂') : Equiv (p := p) (Φ₁ ⬝∧ Φ₂) (Φ₁' ⬝∧ Φ₂') := by
-  simp [Equiv, setOfSatStates, SatState, StateSatisfiable.StateSat, Set.ext_iff] at *
-  intros _ _ _ _ _
-  constructor
-  . rintro ⟨sat₁, sat₂⟩; constructor; exact (h₁ _).1 sat₁; exact (h₂ _).1 sat₂
-  . rintro ⟨sat₁, sat₂⟩; constructor; exact (h₁ _).2 sat₁; exact (h₂ _).2 sat₂
-
-@[simp]
-theorem neg_congr (h : Equiv (p := p) Φ Φ') : Equiv (p := p) (⬝¬Φ) (⬝¬Φ') := by
-  simp [Equiv, setOfSatStates, SatState, StateSatisfiable.StateSat, Set.ext_iff] at *
-  intros _ _ _ _ _
-  constructor
-  . rintro negSat sat; exact negSat ((h _).2 sat)
-  . rintro negSat sat; exact negSat ((h _).1 sat)
-
-@[simp]
-theorem exist_next_congr (h : Equiv (p := p) Φ Φ') : Equiv (p := p) (⬝∃⬝◯Φ) (⬝∃⬝◯Φ') := by
-  simp [Equiv, setOfSatStates, SatState, StateSatisfiable.StateSat, Set.ext_iff] at *
-  intros _ _ _ _ _
-  constructor
-  . rintro ⟨π, sat⟩; exact ⟨π, (h _).1 sat⟩
-  . rintro ⟨π, sat⟩; exact ⟨π, (h _).2 sat⟩
-
-@[simp]
-theorem exist_untl_congr (h₁ : Equiv (p := p) Φ Φ') (h₂ : Equiv (p := p) Ψ Ψ') : Equiv (p := p) (⬝∃(Φ ⬝U Ψ)) (⬝∃(Φ' ⬝U Ψ')) := by
-  simp [Equiv, setOfSatStates, SatState, StateSatisfiable.StateSat, Set.ext_iff] at *
-  intros _ _ _ _ _
-  constructor
-  . rintro ⟨π, j, ⟨satJ, satK⟩⟩; exact ⟨π, j, ⟨(h₂ _).1 satJ, fun k => (h₁ _).1 (satK k)⟩⟩
-  . rintro ⟨π, j, ⟨satJ, satK⟩⟩; exact ⟨π, j, ⟨(h₂ _).2 satJ, fun k => (h₁ _).2 (satK k)⟩⟩
-
-@[simp]
-theorem all_next_congr (h : Equiv (p := p) Φ Φ') : Equiv (p := p) (⬝∀⬝◯Φ) (⬝∀⬝◯Φ') := by
-  simp [Equiv, setOfSatStates, SatState, StateSatisfiable.StateSat, Set.ext_iff] at *
-  intros _ _ _ _ _
-  constructor
-  . rintro sat π; rw [← h]; exact sat π
-  . rintro sat π; rw [h]  ; exact sat π
-  done
-
-@[simp]
-theorem all_untl_congr (h₁ : Equiv (p := p) Φ Φ') (h₂ : Equiv (p := p) Ψ Ψ') : Equiv (p := p) (⬝∀(Φ ⬝U Ψ)) (⬝∀(Φ' ⬝U Ψ')) := by
-  simp [Equiv, setOfSatStates, SatState, StateSatisfiable.StateSat, Set.ext_iff] at *
-  intros _ _ _ _ _
-  constructor
-  . rintro sat π; obtain ⟨j, ⟨satJ, satK⟩⟩ := sat π; exact ⟨j, ⟨(h₂ _).1 satJ, fun k => (h₁ _).1 (satK k)⟩⟩
-  . rintro sat π; obtain ⟨j, ⟨satJ, satK⟩⟩ := sat π; exact ⟨j, ⟨(h₂ _).2 satJ, fun k => (h₁ _).2 (satK k)⟩⟩
-
-theorem all_next_duality : Equiv (p := p) (⬝∀⬝◯Φ) (⬝¬(⬝∃⬝◯⬝¬Φ)) := by
-  simp [Equiv, setOfSatStates, SatState, StateSatisfiable.StateSat, Set.ext_iff] at *
-
-theorem inevitable_duality : Equiv (p := p) (⬝∀♢Φ) (⬝¬(⬝∃■⬝¬Φ)) := by
-  simp [Equiv, setOfSatStates, SatState, StateSatisfiable.StateSat, StateFormula.inevitable, PathFormula.untl]
-
-theorem exist_next_duality : Equiv (p := p) (⬝∃⬝◯Φ) (⬝¬(⬝∀⬝◯⬝¬Φ)) := by
-  simp [Equiv, setOfSatStates, SatState, StateSatisfiable.StateSat]
-
-theorem potential_duality : Equiv (p := p) (⬝∃♢Φ) (⬝¬(⬝∀■⬝¬Φ)) := by
-  simp [Equiv, setOfSatStates, SatState, StateSatisfiable.StateSat, StateFormula.potential, PathFormula.untl]
-
-theorem all_untl_duality : Equiv (p := p) (⬝∀(Φ ⬝U Ψ)) (⬝¬(⬝∃(⬝¬Ψ ⬝U (⬝¬Φ ⬝∧ ⬝¬Ψ))) ⬝∧ ⬝¬(⬝∃■⬝¬Ψ)) := by
-  simp [Equiv, setOfSatStates, SatState, StateSatisfiable.StateSat, Set.ext_iff] at *
-  intros _ _ _ _ _
-  constructor
-  . rintro sat
-    constructor
-    . rintro π j negSatΦ negSatΨ
-      obtain ⟨a, ⟨satΨ, satΦ⟩⟩ := sat π
-      sorry
-    . rintro π
-      obtain ⟨_, ⟨_, _⟩⟩ := sat π
-      constructor <;> assumption
-  . rintro ⟨negSat, satΨ⟩ π
-    obtain ⟨j, satΨ'⟩ := satΨ π
-    exact ⟨j, ⟨satΨ', fun k => sorry⟩⟩
-
-theorem all_untl_expansion : Equiv (p := p) (⬝∀(Φ ⬝U Ψ)) (Ψ ⬝∨ (Φ ⬝∧ (⬝∀⬝◯⬝∀(Φ ⬝U Ψ)))) := by
-  -- simp [Equiv, satStateSet, SatState, StateSat, PathSat, StateFormula.disj]
-  -- intro s a ts
-  -- ext x
-  -- done
-  sorry
-end StateFormula
 end Equiv
-
 end CTL
